refocusing_machine.v
@@ -1,120 +1,111 @@
 
 (*** Signatures ***)
 
-
+Require Import Relations.
+Require Import Entropy.
 Require Import reduction_semantics.
 Require Import refocusing_semantics.
 Require Import abstract_machine.
 
 
 
-Module Type REF_EVAL_APPLY_MACHINE (R : RED_LANG) (RS : RED_REF_SEM R) 
-                                                    <: DET_ABSTRACT_MACHINE.
+Module Type REF_EVAL_APPLY_MACHINE (R : RED_REF_SEM) <: ABSTRACT_MACHINE.
 
   Import R.
-  Import RS.ST.
+  Import ST.
 
+  Notation ick := init_ckind.
 
   Definition term  := term.
-  Definition value := value init_ckind.
+  Definition value := value ick.
 
   Inductive conf : Set :=
-  | c_eval  : term -> forall {k1 k2}, context k1 k2 -> conf
-  | c_apply : forall {k1 k2}, context k1 k2 -> R.value k2 -> conf.
+  | c_eval  : term -> forall {k}, context ick k -> conf
+  | c_apply : forall {k}, context ick k -> R.value k -> conf.
   Definition configuration := conf.
 
-  Definition c_init t            := c_eval t [.](init_ckind).
-  Definition c_final (v : value) := c_apply [.] v.
-  (*Definition final_of (st : configuration) : option value := 
-      match st with 
-      | c_apply k _ [.] v => 
-          match is_initial k with
-          | left H => match H in _ = k return R.value k -> option value with
-                      | eq_refl => fun v => Some v
-                      end v
-          | _      => None
-          end
-      | _ => None
+  Definition load t                    : configuration := c_eval t [.].
+  Definition value_to_conf (v : value) : configuration := c_apply [.] v.
+  Coercion value_to_conf : value >-> configuration.
+  Definition final (c : configuration) : option value := 
+      match c with
+      | c_apply _ [.] v => Some v 
+      | _  => None
       end.
-  Axiom final_of_correct : forall c v, final_of c = Some v <-> c_final v = c.*)
+  Definition decompile (c : configuration) : term :=
+      match c with
+      | c_eval t _ c  => c[t]
+      | c_apply _ c v => c[v]
+      end.
 
 
-  Reserved Notation "st1 → st2" (at level 40, no associativity).
+  Reserved Notation "c1 → c2" (no associativity, at level 70).
 
   Inductive trans : configuration -> configuration -> Prop :=
 
-  | t_red  : forall t {k1 k2} (c : context k1 k2) {r : redex k2} { t0},
-               dec_term t k2 = in_red r -> contract r = Some t0 ->
+  | t_red  : forall t {k} (c : context ick k) r t0,
+               dec_term t k = in_red r -> contract r = Some t0 ->
                c_eval t c → c_eval t0 c
-  | t_val  : forall t {k1 k2} (c : context k1 k2) {v},
-      	       dec_term t k2 = in_val v ->
+  | t_val  : forall t {k} (c : context ick k) v,
+      	       dec_term t k = in_val v ->
                c_eval t c → c_apply c v
-  | t_term : forall t {k1 k2} (c : context k1 k2) {t0 ec},
-               dec_term t k2 = in_term t0 ec ->
+  | t_term : forall t {k} (c : context ick k) {t0 ec},
+               dec_term t k = in_term t0 ec ->
                c_eval t c → c_eval t0 (ec=:c)
-  | t_cred : forall ec {k2} (v : R.value (k2+>ec)) {k1} (c : context k1 k2) {r t},
-               dec_context ec k2 v = in_red r -> contract r = Some t ->
+  | t_cred : forall ec {k} (v : R.value (k+>ec)) (c : context ick k) r t,
+               dec_context ec k v = in_red r -> contract r = Some t ->
                c_apply (ec=:c) v → c_eval t c
-  | t_cval : forall ec {k2} (v : R.value (k2+>ec)) {k1} (c : context k1 k2) {v0},
-               dec_context ec k2 v = in_val v0 ->
+  | t_cval : forall ec {k} (v : R.value (k+>ec)) (c : context ick k) v0,
+               dec_context ec k v = in_val v0 ->
                c_apply (ec=:c) v → c_apply c v0
-  | t_cterm: forall ec {k2} (v : R.value (k2+>ec)) {k1} (c : context k1 k2) {t ec0},
-               dec_context ec k2 v = in_term t ec0 ->
+  | t_cterm: forall ec {k} (v : R.value (k+>ec)) (c : context ick k) t ec0,
+               dec_context ec k v = in_term t ec0 ->
                c_apply (ec=:c) v → c_eval t (ec0=:c)
 
   where "st1 → st2" := (trans st1 st2).
   Definition transition := trans.
   Hint Unfold transition.
 
-  Axiom final_correct : forall v st, ~ c_final v → st.
+  Notation "t1 →+ t2" := (clos_trans_1n _ transition t1 t2) 
+                                                         (no associativity, at level 70).
+  Notation "t1 →* t2" := (clos_refl_trans_1n _ transition t1 t2) 
+                                                         (no associativity, at level 70).
 
 
-
-  Reserved Notation "c1 →+ c2" (at level 40, no associativity).
-  Reserved Notation "c1 →* c2" (at level 40, no associativity).
-
-  Inductive trans_close : configuration -> configuration -> Prop :=
-  | one_step   : forall c1 c2,     c1 → c2  ->  c1 →+ c2
-  | multi_step : forall c1 c2 c3,  c1 → c2  ->  c2 →+ c3  ->  c1 →+ c3
-  where "c1 →+ c2" := (trans_close c1 c2).
-
-  Definition trans_ref_close c1 c2 := c1 = c2 \/ trans_close c1 c2.
-  Notation "c1 →* c2" := (trans_ref_close c1 c2).
-
-
-  Inductive eval : term -> value -> Prop :=
-  | e_intro : forall t v, trans_close (c_init t) (c_final v) -> eval t v.
-
-
-  Definition next_conf st :=
+  Definition next_conf (_ : entropy) st :=
       match st with
-      | c_eval t _ k2 c  => 
-            match dec_term t k2 with
+      | c_eval t k c  => 
+            match dec_term t k with
             | in_red r => option_map (fun t' => c_eval t' c) (contract r)
             | in_val v => Some (c_apply c v)
             | in_term t ec => Some (c_eval t (ec=:c))
             | in_dead => None
             end
-      | c_apply _ _ (ccons ec k c) v => 
+      | c_apply _ (ccons ec k c) v => 
             match dec_context ec k v with
             | in_red r => option_map (fun t' => c_eval t' c) (contract r)
             | in_val v => Some (c_apply c v)
             | in_term t ec => Some (c_eval t (ec=:c))
             | in_dead => None
             end
-      | c_apply _ _ [.] v => 
+      | c_apply _ [.] v => 
             None
       end.
 
-
-  Axiom next_correct  : forall c1 c2, next_conf c1 = Some c2 <-> c1 → c2.
+  Axioms
+  (final_correct :                                                              forall c,
+       final c <> None -> ~exists c', c → c')
+  (trans_computable :                                                       forall c1 c2,
+       c1 → c2 <-> exists e, next_conf e c1 = Some c2)
+  (finals_are_vals :                                                          forall c v,
+       final c = Some v <-> c = v).
 
 End REF_EVAL_APPLY_MACHINE.
 
 
 
 
-
+(*
 Module Type REF_PUSH_ENTER_MACHINE (R : RED_LANG) (PERS : PE_RED_REF_SEM R) 
                                                        <: DET_ABSTRACT_MACHINE.
 
@@ -218,7 +209,7 @@ Module Type REF_PUSH_ENTER_MACHINE (R : RED_LANG) (PERS : PE_RED_REF_SEM R)
 
   Axiom next_correct  : forall c1 c2, next_conf c1 = Some c2 <-> c1 → c2.
 
-End REF_PUSH_ENTER_MACHINE.
+End REF_PUSH_ENTER_MACHINE.*)
 
 
 
@@ -233,104 +224,121 @@ Require Export reduction_strategy.
 
 
 
-Module RefEvalApplyMachine (R : RED_LANG) (RS : RED_REF_SEM R) 
-                                                 <: REF_EVAL_APPLY_MACHINE R RS.
+Module RefEvalApplyMachine (R : RED_REF_SEM) <: REF_EVAL_APPLY_MACHINE R.
 
   Import R.
-  Import RS.ST.
+  Import ST.
+
+  Notation ick := init_ckind.
 
 
   Definition term  := term.
-  Definition value := value init_ckind.
+  Definition value := value ick.
 
   Inductive conf : Set :=
-  | c_eval  : term -> forall {k1 k2}, context k1 k2 -> conf
-  | c_apply : forall {k1 k2}, context k1 k2 -> R.value k2 -> conf.
+  | c_eval  : term -> forall {k}, context ick k -> conf
+  | c_apply : forall {k}, context ick k -> R.value k -> conf.
   Definition configuration := conf.
 
-  Definition c_init t            := c_eval t [.](init_ckind).
-  Definition c_final (v : value) := c_apply [.] v.
+  Definition load t                    : configuration := c_eval t [.].
+  Definition value_to_conf (v : value) : configuration := c_apply [.] v.
+  Coercion value_to_conf : value >-> configuration.
+  Definition final (c : configuration) : option value := 
+      match c with
+      | c_apply _ [.] v => Some v 
+      | _  => None
+      end.
+  Definition decompile (c : configuration) : term :=
+      match c with
+      | c_eval t _ c  => c[t]
+      | c_apply _ c v => c[v]
+      end.
 
 
-  Reserved Notation "c1 → c2" (at level 40, no associativity).
+  Reserved Notation "c1 → c2" (no associativity, at level 70).
 
   Inductive trans : configuration -> configuration -> Prop :=
 
-  | t_red  : forall t {k1 k2} (c : context k1 k2) {r : redex k2} {t0},
-               dec_term t k2 = in_red r -> contract r = Some t0 ->
+  | t_red  : forall t {k} (c : context ick k) r t0,
+               dec_term t k = in_red r -> contract r = Some t0 ->
                c_eval t c → c_eval t0 c
-  | t_val  : forall t {k1 k2} (c : context k1 k2) {v},
-      	       dec_term t k2 = in_val v ->
+  | t_val  : forall t {k} (c : context ick k) v,
+      	       dec_term t k = in_val v ->
                c_eval t c → c_apply c v
-  | t_term : forall t {k1 k2} (c : context k1 k2) {t0 ec},
-               dec_term t k2 = in_term t0 ec ->
+  | t_term : forall t {k} (c : context ick k) {t0 ec},
+               dec_term t k = in_term t0 ec ->
                c_eval t c → c_eval t0 (ec=:c)
-  | t_cred : forall ec {k2} (v : R.value (k2+>ec)) {k1} (c : context k1 k2) {r t},
-               dec_context ec k2 v = in_red r -> contract r = Some t ->
+  | t_cred : forall ec {k} (v : R.value (k+>ec)) (c : context ick k) r t,
+               dec_context ec k v = in_red r -> contract r = Some t ->
                c_apply (ec=:c) v → c_eval t c
-  | t_cval : forall ec {k2} (v : R.value (k2+>ec)) {k1} (c : context k1 k2) {v0},
-               dec_context ec k2 v = in_val v0 ->
+  | t_cval : forall ec {k} (v : R.value (k+>ec)) (c : context ick k) v0,
+               dec_context ec k v = in_val v0 ->
                c_apply (ec=:c) v → c_apply c v0
-  | t_cterm: forall ec {k2} (v : R.value (k2+>ec)) {k1} (c : context k1 k2) {t ec0},
-               dec_context ec k2 v = in_term t ec0 ->
+  | t_cterm: forall ec {k} (v : R.value (k+>ec)) (c : context ick k) t ec0,
+               dec_context ec k v = in_term t ec0 ->
                c_apply (ec=:c) v → c_eval t (ec0=:c)
 
-  where "c1 → c2" := (trans c1 c2).
+  where "st1 → st2" := (trans st1 st2).
   Definition transition := trans.
   Hint Unfold transition.
 
-
-  Lemma final_correct : forall v st, ~ c_final v → st.
-
-  Proof. inversion 1. Qed.
-
-
-  Reserved Notation "c1 →+ c2" (at level 40, no associativity).
-  Reserved Notation "c1 →* c2" (at level 40, no associativity).
-
-  Inductive trans_close : configuration -> configuration -> Prop :=
-  | one_step   : forall c1 c2,     c1 → c2  ->  c1 →+ c2
-  | multi_step : forall c1 c2 c3,  c1 → c2  ->  c2 →+ c3  ->  c1 →+ c3
-  where "c1 →+ c2" := (trans_close c1 c2).
-
-  Definition trans_ref_close c1 c2 := c1 = c2 \/ trans_close c1 c2.
-  Notation "c1 →* c2" := (trans_ref_close c1 c2).
+  Notation "t1 →+ t2" := (clos_trans_1n _ transition t1 t2) 
+                                                         (no associativity, at level 70).
+  Notation "t1 →* t2" := (clos_refl_trans_1n _ transition t1 t2) 
+                                                         (no associativity, at level 70).
 
 
-  Inductive eval : term -> value -> Prop :=
-  | e_intro : forall t v, trans_close (c_init t) (c_final v) -> eval t v.
-
-
-  Definition next_conf st :=
+  Definition next_conf (_ : entropy) st :=
       match st with
-      | c_eval t _ k2 c  => 
-            match dec_term t k2 with
+      | c_eval t k c  => 
+            match dec_term t k with
             | in_red r => option_map (fun t' => c_eval t' c) (contract r)
             | in_val v => Some (c_apply c v)
             | in_term t ec => Some (c_eval t (ec=:c))
             | in_dead => None
             end
-      | c_apply _ _ (ccons ec k c) v => 
+      | c_apply _ (ccons ec k c) v => 
             match dec_context ec k v with
             | in_red r => option_map (fun t' => c_eval t' c) (contract r)
             | in_val v => Some (c_apply c v)
             | in_term t ec => Some (c_eval t (ec=:c))
             | in_dead => None
             end
-      | c_apply _ _ [.] v => 
+      | c_apply _ [.] v => 
             None
       end.
 
 
+  Lemma final_correct :                                                         forall c,
+       final c <> None -> ~exists c', c → c'.
 
-  Lemma next_correct : forall c1 c2, next_conf c1 = Some c2 <-> c1 → c2.
+  Proof.
+    intros c H [c' H0].
+    inversion H0; subst;
+        simpl in H;
+    congruence.
+  Qed.
 
+
+  Lemma trans_computable :                                                  forall c1 c2,
+       c1 → c2 <-> exists e, next_conf e c1 = Some c2.
   Proof.
     intros c1 c2; split; intro H.
 
   (* -> *) {
+      destruct (draw_fin_correct 1 Fin.F1) as [ent _].
+      destruct H;
+          simpl;
+          match goal with H : @eq (interm_dec _) _ _ |- _ => rewrite H end;
+      solve 
+      [ eauto 
+      | rewrite H0; eauto].
+  }
+
+  (* <- *) {
+      destruct H as [ent H].
       destruct c1; simpl in H.
-      - remember (dec_term t k2) as dc.
+      - remember (dec_term t k) as dc.
         destruct dc.
         + remember (contract r) as opt.
           destruct opt.
@@ -356,15 +364,20 @@ Module RefEvalApplyMachine (R : RED_LANG) (RS : RED_REF_SEM R)
           apply t_cval; auto.
         + inversion H.
   }
+  Qed.
 
-  (* <- *) {
-      destruct H;
-          simpl;
-          match goal with H : @eq (interm_dec _) _ _ |- _ => rewrite H end;
-      solve 
-      [ auto 
-      | rewrite H0; auto].
-  }
+
+  Lemma finals_are_vals :                                                     forall c v,
+       final c = Some v <-> c = v.
+  Proof.
+    intros c v.
+    destruct c; simpl.
+    - intuition.
+    - destruct c.
+      + split; intro H;
+            inversion H; dep_subst;
+        solve [auto].
+      + intuition.
   Qed.
 
 End RefEvalApplyMachine.
@@ -372,7 +385,7 @@ End RefEvalApplyMachine.
 
 
 
-Module RefPushEnterMachine (R : RED_LANG) (PERS : PE_RED_REF_SEM R) 
+(*Module RefPushEnterMachine (R : RED_LANG) (PERS : PE_RED_REF_SEM R) 
                                                  <: REF_PUSH_ENTER_MACHINE R PERS.
 
   Import R.
@@ -505,4 +518,4 @@ Module RefPushEnterMachine (R : RED_LANG) (PERS : PE_RED_REF_SEM R)
   }
   Qed.
 
-End RefPushEnterMachine.
+End RefPushEnterMachine.*)
