refocusing_natural_semantics.v
@@ -7,27 +7,26 @@ Require Import refocusing_semantics.
 
 
 
+Module Type REF_EVALUATOR (R : RED_REF_SEM).
 
-Module Type PRE_REF_NATURAL_SEM (R : RED_LANG) (RS : RED_REF_SEM R).
-
-  Module ST := RS.ST.
-  Export ST.
   Import R.
+  Export ST.
 
 
-  Inductive dec : term -> forall {k1 k2}, context k1 k2 -> decomp k1 -> Prop :=
+  (*
+  Inductive dec' : term -> forall {k1 k2}, context k1 k2 -> decomp k1 -> Prop :=
 
   | d_dec  : forall t {k1 k2} (c : context k1 k2) {r},
                dec_term t k2 = in_red r -> 
-               dec t c (d_red r c)
+               dec' t c (d_red r c)
   | d_v    : forall t {k1 k2} {c : context k1 k2} {v d},
                dec_term t k2 = in_val v ->
                decctx v c d ->
-               dec t c d
+               dec' t c d
   | d_term : forall t {t0 k1 k2} {c : context k1 k2} {ec d},
                dec_term t k2 = in_term t0 ec ->
-               dec t0 (ec=:c) d ->
-               dec t c d
+               dec' t0 (ec=:c) d ->
+               dec' t c d
 
   with decctx : forall {k2}, value k2 -> 
                     forall {k1}, context k1 k2 -> decomp k1 -> Prop :=
@@ -46,151 +45,111 @@ Module Type PRE_REF_NATURAL_SEM (R : RED_LANG) (RS : RED_REF_SEM R).
   | dc_term : forall ec {ec0 k2} (v : value (k2+>ec)) 
                             {k1} {c : context k1 k2} {t d},
                 dec_context ec k2 v = in_term t ec0 ->
-                dec t (ec0=:c) d ->
+                dec' t (ec0=:c) d ->
                 decctx v (ec=:c) d.
-
-  Scheme dec_Ind    := Induction for dec Sort Prop
-    with decctx_Ind := Induction for decctx Sort Prop.
-
-
-  Inductive iter : forall {k}, decomp k -> value k -> Prop :=
-  | i_val : forall {k} (v : value k), 
-              iter (d_val v) v
-  | i_red : forall {k2} (r : redex k2) {t k1} {c : context k1 k2} {d v},
-              contract r = Some t  ->  dec t c d  ->  iter d v ->
-              iter (d_red r c) v.
-
-
-  Inductive eval : term -> value init_ckind -> Prop :=
-  | e_intro : forall {t d v}, dec t [.] d -> iter d v -> eval t v.
-
-End PRE_REF_NATURAL_SEM.
+  *)
 
 
 
+  (* The evaluation function that is going to be realized :
+     Fixpoint eval k t := 
+         match dec_fun t [.](k) with
+         | d_val v   => v
+         | d_red r c => match contract r with
+                        | None    => undefined
+                        | Some t' => eval k c[t]
+                        end
+         end. *)
+  Inductive eval k t : value k -> Prop :=
+  | e_val : forall {v}, 
+                dec_proc t [.](k) (d_val v) -> eval k t v
+  | e_red : forall {k'} {c : context k k'} {r t' v}, 
+                dec_proc t [.](k) (d_red r c) -> 
+                contract r = Some t'     ->
+                eval k c[t'] v           ->
+                eval k t v.
 
 
-Module Type STAGED_REF_NATURAL_SEM (R : RED_LANG) (RS : RED_REF_SEM R).
+  Axiom evalRS_imp_eval :                                    forall  {k t} {v : value k},
+      ~dead_ckind k  ->  (k |~ t →* v)  ->  eval k t v.
+  Axiom eval_eqv_RS :                                                     forall {k t v},
+      eval k t v  <->  ~dead_ckind k /\ (k |~ t →* v).
 
-  Module ST := RS.ST.
+End REF_EVALUATOR.
+
+
+
+
+Module Type REF_NATURAL_SEM (R : RED_REF_SEM).
+
   Import R.
   Export ST.
 
 
-  Inductive dec : term -> forall {k1 k2}, context k1 k2 -> value k1 -> Prop :=
+  Inductive dec_eval : 
+      term -> forall {k1 k2}, context k1 k2 -> value k1 -> Prop :=
 
-  | d_dec  : forall t {k1 k2} {c : context k1 k2} {r v},
-               dec_term t k2 = in_red r -> 
-               iter (d_red r c) v ->
-               dec t c v
-  | d_v    : forall t {k1 k2} {c : context k1 k2} {v v0},
-               dec_term t k2 = in_val v -> 
-               decctx v c v0 ->
-               dec t c v0
-  | d_many : forall t {t0 ec k1 k2} {c : context k1 k2} {v},
-               dec_term t k2 = in_term t0 ec -> 
-               dec t0 (ec=:c) v ->
-               dec t c v
+  | de_dec  : forall t {t0 k1 k2} {c : context k1 k2} {r : redex k2} {v},
+                  dec_term t k2 = in_red r -> 
+                  contract r = Some t0 -> 
+                  dec_eval t0 c v ->
+                  dec_eval t c v
+  | de_v    : forall t {k1 k2} {c : context k1 k2} {v v0},
+                  dec_term t k2 = in_val v -> 
+                  decctx_eval v c v0 ->
+                  dec_eval t c v0
+  | de_term : forall t {t0 ec k1 k2} {c : context k1 k2} {v},
+                  dec_term t k2 = in_term t0 ec -> 
+                  dec_eval t0 (ec=:c) v ->
+                  dec_eval t c v
 
-  with decctx : forall {k2}, value k2 -> 
-                    forall {k1}, context k1 k2 -> value k1 -> Prop :=
+  with decctx_eval : forall {k2}, value k2 -> 
+                         forall {k1}, context k1 k2 -> value k1 -> Prop :=
 
-  | dc_end  : forall {k} {v v0 : value k},
-                ~ dead_ckind k ->
-                iter (d_val v) v0 ->
-                decctx v [.] v0
-  | dc_dec  : forall ec {k2} (v : value (k2+>ec)) {k1} {c : context k1 k2} {r v0},
-                dec_context ec k2 v = in_red r -> 
-                iter (d_red r c) v0 ->
-                decctx v (ec=:c) v0
-  | dc_val  : forall ec {k2} (v : value (k2+>ec)) {v0 k1} {c : context k1 k2} {v1},
-                dec_context ec k2 v = in_val v0 -> 
-                decctx v0 c v1 ->
-                decctx v (ec=:c) v1
-  | dc_term : forall ec {k2} (v : value (k2+>ec)) {t ec0 k1} {c : context k1 k2} {v0},
-                dec_context ec k2 v = in_term t ec0 -> 
-                dec t (ec0=:c) v0 ->
-                decctx v (ec=:c) v0
+  | dce_end  : forall {k} (v : value k), 
+                   ~ dead_ckind k ->
+                   decctx_eval v [.] v
+  | dce_dec  : forall ec {k2} (v0 : value (k2+>ec)) {k1} (c : context k1 k2) {r t v1},
+                   dec_context ec k2 v0 = in_red r ->
+                   contract r = Some t             ->
+                   dec_eval t c v1                 ->
+                   decctx_eval v0 (ec=:c) v1
+  | dce_val  : forall {k2} {v1 : value k2} ec (v0 : value (k2+>ec)) 
+                     {k1} {c  : context k1 k2} {v2},
+                   dec_context ec k2 v0 = in_val v1 ->
+                   decctx_eval v1 c v2 ->
+                   decctx_eval v0 (ec=:c) v2
+  | dce_term : forall ec {ec0 k2} (v0 : value (k2+>ec)) 
+                            {k1} {c : context k1 k2} {t v1},
+                   dec_context ec k2 v0 = in_term t ec0 ->
+                   dec_eval t (ec0=:c) v1 ->
+                   decctx_eval v0 (ec=:c) v1.
 
-  with iter : forall {k}, decomp k -> value k -> Prop :=
-
-  | i_val : forall {k} (v : value k), 
-              iter (d_val v) v
-  | i_red : forall {k2} (r : redex k2) {k1} {c : context k1 k2} {t v},
-              contract r = Some t -> 
-              dec t c v -> 
-              iter (d_red r c) v.
-
-  Scheme dec_Ind    := Induction for dec Sort Prop
-    with decctx_Ind := Induction for decctx Sort Prop
-    with iter_Ind   := Induction for iter Sort Prop.
+  Scheme dec_eval_Ind    := Induction for dec_eval    Sort Prop
+    with decctx_eval_Ind := Induction for decctx_eval Sort Prop.
 
 
-  Inductive eval : term -> value init_ckind -> Prop :=
-  | e_intro : forall {t v}, dec t [.] v -> eval t v.
-
-End STAGED_REF_NATURAL_SEM.
+  Definition eval k t v := dec_eval t [.](k) v.
 
 
 
+  Axioms
+  (dec_evalRS_imp_dec_eval :         forall t {k1 k2} (v : value k1) (c : context k1 k2),
+       ~dead_ckind k2  ->  (k1 |~ c[t] →* v)  ->  dec_eval t c v)
+  (dec_eval_eqv_RS :                 forall t {k1 k2} (v : value k1) (c : context k1 k2),
+          dec_eval t c v  <->  ~dead_ckind k1 /\ (k1 |~ c[t] →* v))
 
-
-Module Type REF_NATURAL_SEM (R : RED_LANG) (RS : RED_REF_SEM R).
-
-  Module ST := RS.ST.
-  Export ST.
-  Import R.
-
-
-  Inductive dec : term -> forall {k1 k2}, context k1 k2 -> value k1 -> Prop :=
-
-  | d_d_r  : forall t {t0 k1 k2} {c : context k1 k2} {r : redex k2} {v},
-               dec_term t k2 = in_red r -> 
-               contract r = Some t0 -> 
-               dec t0 c v ->
-               dec t c v
-  | d_v    : forall t {k1 k2} {c : context k1 k2} {v v0},
-               dec_term t k2 = in_val v -> 
-               decctx v c v0 ->
-               dec t c v0
-  | d_term : forall t {t0 ec k1 k2} {c : context k1 k2} {v},
-               dec_term t k2 = in_term t0 ec -> 
-               dec t0 (ec=:c) v ->
-               dec t c v
-
-  with decctx : forall {k2}, value k2 -> 
-                    forall {k1}, context k1 k2 -> value k1 -> Prop :=
-
-  | dc_end : forall {k} (v : value k), 
-               ~ dead_ckind k ->
-               decctx v [.] v
-  | dc_red : forall ec {k2} (v : value (k2+>ec)) {k1} {c : context k1 k2} {r t v0},
-               dec_context ec k2 v = in_red r -> 
-               contract r = Some t -> 
-               dec t c v0 ->
-               decctx v (ec=:c) v0
-  | dc_rec : forall ec {k2} (v : value (k2+>ec)) {k1} {c : context k1 k2} {v0 v1},
-               dec_context ec k2 v = in_val v0 -> 
-               decctx v0 c v1 ->
-               decctx v (ec=:c) v1
-  | dc_trm : forall ec {k2} (v : value (k2+>ec)) {k1} {c : context k1 k2} {t ec0 v0},
-               dec_context ec k2 v = in_term t ec0 -> 
-               dec t (ec0=:c) v0 ->
-               decctx v (ec=:c) v0.
-
-  Scheme dec_Ind    := Induction for dec Sort Prop
-    with decctx_Ind := Induction for decctx Sort Prop.
-
-
-  Inductive eval : term -> value init_ckind -> Prop :=
-  | e_intro : forall {t v}, dec t [.] v -> eval t v.
+  (evalRS_imp_eval :                                         forall  {k t} {v : value k},
+      ~dead_ckind k  ->  (k |~ t →* v)  ->  eval k t v)
+  (eval_eqv_RS :                                                          forall {k t v},
+      eval k t v  <->  ~dead_ckind k /\ (k |~ t →* v)).
 
 End REF_NATURAL_SEM.
 
 
 
 
-
+(*
 Module Type PE_REF_NATURAL_SEM (R : RED_LANG) (PERS : PE_RED_REF_SEM R).
 
   Module ST := PERS.ST.
@@ -236,7 +195,7 @@ Module Type PE_REF_NATURAL_SEM (R : RED_LANG) (PERS : PE_RED_REF_SEM R).
   Inductive eval : term -> value init_ckind -> Prop :=
   | e_intro : forall {t v}, dec t [.] v -> eval t v.
 
-End PE_REF_NATURAL_SEM.
+End PE_REF_NATURAL_SEM.*)
 
 
 
@@ -245,183 +204,242 @@ End PE_REF_NATURAL_SEM.
 (*** Functors ***)
 
 
-Require Import Util.
 Require Export reduction_strategy.
+Require Import 
+    Program 
+    Util
+    reduction_languages_facts 
+    reduction_semantics_facts 
+    refocusing_semantics_facts.
 
 
 
-Module PreRefNaturalSem (R : RED_LANG) (RS : RED_REF_SEM R) 
-                                                <: PRE_REF_NATURAL_SEM R RS.
+Module RefEvaluator (R : RED_REF_SEM) <: REF_EVALUATOR R.
 
-  Module ST := RS.ST.
-  Export ST.
-  Import R.
-
-
-  Inductive dec : term -> forall {k1 k2}, context k1 k2 -> decomp k1 -> Prop :=
-
-  | d_dec  : forall t {k1 k2} (c : context k1 k2) {r},
-               dec_term t k2 = in_red r -> 
-               dec t c (d_red r c)
-  | d_v    : forall t {k1 k2} {c : context k1 k2} {v d},
-               dec_term t k2 = in_val v ->
-               decctx v c d ->
-               dec t c d
-  | d_term : forall t {t0 k1 k2} {c : context k1 k2} {ec d},
-               dec_term t k2 = in_term t0 ec ->
-               dec t0 (ec=:c) d ->
-               dec t c d
-
-  with decctx : forall {k2}, value k2 -> 
-                    forall {k1}, context k1 k2 -> decomp k1 -> Prop :=
-
-  | dc_end  : forall {k} (v : value k), 
-                ~ dead_ckind k ->
-                decctx v [.] (d_val v)
-  | dc_dec  : forall ec {k2} (v : value (k2+>ec)) {k1} (c : context k1 k2) {r},
-                dec_context ec k2 v = in_red r ->
-                decctx v (ec=:c) (d_red r c)
-  | dc_val  : forall {k2} {v0 : value k2} ec (v : value (k2+>ec)) 
-                     {k1} {c  : context k1 k2} {d},
-                dec_context ec k2 v = in_val v0 ->
-                decctx v0 c d ->
-                decctx v (ec=:c) d
-  | dc_term : forall ec {ec0 k2} (v : value (k2+>ec)) 
-                            {k1} {c : context k1 k2} {t d},
-                dec_context ec k2 v = in_term t ec0 ->
-                dec t (ec0=:c) d ->
-                decctx v (ec=:c) d.
-
-  Scheme dec_Ind    := Induction for dec Sort Prop
-    with decctx_Ind := Induction for decctx Sort Prop.
-
-
-  Inductive iter : forall {k}, decomp k -> value k -> Prop :=
-  | i_val : forall {k} (v : value k), 
-              iter (d_val v) v
-  | i_red : forall {k2} (r : redex k2) {t k1} {c : context k1 k2} {d v},
-              contract r = Some t -> 
-              dec t c d -> 
-              iter d v ->
-              iter (d_red r c) v.
-
-
-  Inductive eval : term -> value init_ckind -> Prop :=
-  | e_intro : forall {t d v}, dec t [.] d -> iter d v -> eval t v.
-
-End PreRefNaturalSem.
-
-
-
-
-Module StagedRefNaturalSem (R : RED_LANG) (RS : RED_REF_SEM R) 
-                                                <: STAGED_REF_NATURAL_SEM R RS.
-
-  Module ST := RS.ST.
-  Import R.
+  Module RLF := RED_LANG_Facts R.
+  Module RF  := RED_REF_SEM_Facts R.
+  Module RD  := RedRefSemDet R.
+  Import R RLF RF RD.
   Export ST.
 
 
-  Inductive dec : term -> forall {k1 k2}, context k1 k2 -> value k1 -> Prop :=
-
-  | d_dec  : forall t {k1 k2} {c : context k1 k2} {r v},
-               dec_term t k2 = in_red r -> 
-               iter (d_red r c) v ->
-               dec t c v
-  | d_v    : forall t {k1 k2} {c : context k1 k2} {v v0},
-               dec_term t k2 = in_val v -> 
-               decctx v c v0 ->
-               dec t c v0
-  | d_many : forall t {t0 ec k1 k2} {c : context k1 k2} {v},
-               dec_term t k2 = in_term t0 ec -> 
-               dec t0 (ec=:c) v ->
-               dec t c v
-
-  with decctx : forall {k2}, value k2 -> 
-                    forall {k1}, context k1 k2 -> value k1 -> Prop :=
-
-  | dc_end  : forall {k} {v v0 : value k},
-                ~ dead_ckind k ->
-                iter (d_val v) v0 ->
-                decctx v [.] v0
-  | dc_dec  : forall ec {k2} (v : value (k2+>ec)) {k1} {c : context k1 k2} {r v0},
-                dec_context ec k2 v = in_red r -> 
-                iter (d_red r c) v0 ->
-                decctx v (ec=:c) v0
-  | dc_val  : forall ec {k2} (v : value (k2+>ec)) {v0 k1} {c : context k1 k2} {v1},
-                dec_context ec k2 v = in_val v0 -> 
-                decctx v0 c v1 ->
-                decctx v (ec=:c) v1
-  | dc_term : forall ec {k2} (v : value (k2+>ec)) {t ec0 k1} {c : context k1 k2} {v0},
-                dec_context ec k2 v = in_term t ec0 -> 
-                dec t (ec0=:c) v0 ->
-                decctx v (ec=:c) v0
-
-  with iter : forall {k}, decomp k -> value k -> Prop :=
-
-  | i_val : forall {k} (v : value k), 
-              iter (d_val v) v
-  | i_red : forall {k2} (r : redex k2) {k1} {c : context k1 k2} {t v},
-              contract r = Some t -> 
-              dec t c v -> 
-              iter (d_red r c) v.
-
-  Scheme dec_Ind    := Induction for dec    Sort Prop
-    with decctx_Ind := Induction for decctx Sort Prop
-    with iter_Ind   := Induction for iter   Sort Prop.
-
-
-  Inductive eval : term -> value init_ckind -> Prop :=
-  | e_intro : forall {t v}, dec t [.] v -> eval t v.
-
-End StagedRefNaturalSem.
+  Inductive eval k t : value k -> Prop :=
+  | e_val : forall {v}, 
+                dec_proc t [.](k) (d_val v) -> eval k t v
+  | e_red : forall {k'} {c : context k k'} {r t' v}, 
+                dec_proc t [.](k) (d_red r c) -> 
+                contract r = Some t'     ->
+                eval k c[t'] v           ->
+                eval k t v.
 
 
 
+  Local Hint Constructors dec_proc decctx_proc eval.
 
-Module RefNaturalSem (R : RED_LANG) (RS : RED_REF_SEM R)
-                                              <: REF_NATURAL_SEM R RS.
+  Lemma eval_imp_RS :                                                     forall {k} t v,
+      eval k t v  ->  (k |~ t →* v).
 
-  Module ST := RS.ST.
+  Proof with eauto using dec_proc_starts_alive.
+    intros k t v E.
+    dependent induction E.
+    - apply dec_proc_eqv_dec in H...
+      destruct H.
+      simpl in H0; subst.
+      constructor 1.
+    - constructor 2 with (y:=c[t'])...
+      exists k' c r t'.
+      intuition.
+      rewrite <- plug_empty with t k.
+      apply dec_proc_eqv_dec...
+  Qed.
+
+
+  Lemma evalRS_imp_eval :                                     forall {k} t (v : value k),
+      ~dead_ckind k  ->  (k |~ t →* v)  ->  eval k t v.
+
+  Proof with eauto.
+    intros k t v H H0.
+    dependent induction H0. 
+    - constructor 1.
+      apply dec_proc_eqv_dec...
+      constructor...
+    - destruct H1 as [k' [c [r [t' [? [? ?]]]]]].
+      subst.
+      constructor 2 with k' c r t'...
+      apply dec_proc_eqv_dec...
+  Qed.
+
+
+  Theorem eval_eqv_RS :                                                   forall {k} t v,
+      eval k t v  <->  ~dead_ckind k /\ (k |~ t →* v).
+
+  Proof.
+    intuition eauto using evalRS_imp_eval, eval_imp_RS.
+    destruct H;
+    (
+        assert (H' := dec_term_from_dead t k H0);
+        dependent destruction H; 
+        congruence
+    ).
+  Qed.
+
+End RefEvaluator.
+
+
+
+
+Module RefNaturalSem (R : RED_REF_SEM) <: REF_NATURAL_SEM R.
+
+  Module RF := RED_LANG_Facts R.
+  Import R RF.
   Export ST.
-  Import R.
 
 
-  Inductive dec : term -> forall {k1 k2}, context k1 k2 -> value k1 -> Prop :=
+  Inductive dec_eval : 
+      term -> forall {k1 k2}, context k1 k2 -> value k1 -> Prop :=
 
-  | d_d_r  : forall t {t0 k1 k2} {c : context k1 k2} {r : redex k2} {v},
-               dec_term t k2 = in_red r -> 
-               contract r = Some t0 -> 
-               dec t0 c v ->
-               dec t c v
-  | d_v    : forall t {k1 k2} {c : context k1 k2} {v v0},
-               dec_term t k2 = in_val v -> 
-               decctx v c v0 ->
-               dec t c v0
-  | d_term : forall t {t0 ec k1 k2} {c : context k1 k2} {v},
-               dec_term t k2 = in_term t0 ec -> 
-               dec t0 (ec=:c) v ->
-               dec t c v
+  | de_dec  : forall t {t0 k1 k2} {c : context k1 k2} {r : redex k2} {v},
+                  dec_term t k2 = in_red r -> 
+                  contract r = Some t0 -> 
+                  dec_eval t0 c v ->
+                  dec_eval t c v
+  | de_v    : forall t {k1 k2} {c : context k1 k2} {v v0},
+                  dec_term t k2 = in_val v -> 
+                  decctx_eval v c v0 ->
+                  dec_eval t c v0
+  | de_term : forall t {t0 ec k1 k2} {c : context k1 k2} {v},
+                  dec_term t k2 = in_term t0 ec -> 
+                  dec_eval t0 (ec=:c) v ->
+                  dec_eval t c v
 
-  with decctx : forall {k2}, value k2 -> 
-                    forall {k1}, context k1 k2 -> value k1 -> Prop :=
+  with decctx_eval : forall {k2}, value k2 -> 
+                         forall {k1}, context k1 k2 -> value k1 -> Prop :=
 
-  | dc_end : forall {k} (v : value k), 
-               ~ dead_ckind k ->
-               decctx v [.] v
-  | dc_red : forall ec {k2} (v : value (k2+>ec)) {k1} {c : context k1 k2} {r t v0},
-               dec_context ec k2 v = in_red r -> 
-               contract r = Some t -> 
-               dec t c v0 ->
-               decctx v (ec=:c) v0
-  | dc_rec : forall ec {k2} (v : value (k2+>ec)) {k1} {c : context k1 k2} {v0 v1},
-               dec_context ec k2 v = in_val v0 -> 
-               decctx v0 c v1 ->
-               decctx v (ec=:c) v1
-  | dc_trm : forall ec {k2} (v : value (k2+>ec)) {k1} {c : context k1 k2} {t ec0 v0},
-               dec_context ec k2 v = in_term t ec0 -> 
-               dec t (ec0=:c) v0 ->
-               decctx v (ec=:c) v0.
+  | dce_end  : forall {k} (v : value k), 
+                   ~ dead_ckind k ->
+                   decctx_eval v [.] v
+  | dce_dec  : forall ec {k2} (v0 : value (k2+>ec)) {k1} (c : context k1 k2) {r t v1},
+                   dec_context ec k2 v0 = in_red r ->
+                   contract r = Some t             ->
+                   dec_eval t c v1                 ->
+                   decctx_eval v0 (ec=:c) v1
+  | dce_val  : forall {k2} {v1 : value k2} ec (v0 : value (k2+>ec)) 
+                     {k1} {c  : context k1 k2} {v2},
+                   dec_context ec k2 v0 = in_val v1 ->
+                   decctx_eval v1 c v2 ->
+                   decctx_eval v0 (ec=:c) v2
+  | dce_term : forall ec {ec0 k2} (v0 : value (k2+>ec)) 
+                            {k1} {c : context k1 k2} {t v1},
+                   dec_context ec k2 v0 = in_term t ec0 ->
+                   dec_eval t (ec0=:c) v1 ->
+                   decctx_eval v0 (ec=:c) v1.
+
+  Scheme dec_eval_Ind    := Induction for dec_eval    Sort Prop
+    with decctx_eval_Ind := Induction for decctx_eval Sort Prop.
+
+
+  Definition eval k t v := dec_eval t [.](k) v.
+
+
+
+  Module RE := RefEvaluator R.
+
+  Local Hint Constructors dec_proc decctx_proc RE.eval dec_eval decctx_eval.
+
+
+  Lemma dec_eval_imp_evalRE :                     forall t {k1 k2} v (c : context k1 k2),
+     dec_eval t c v -> RE.eval k1 c[t] v.
+
+  Proof with eauto using (proper_death2 [.]), dead_context_dead.
+    intros t k1 k2 v c H.
+    induction H using dec_eval_Ind with
+    (P  := fun t k1 _ c v _                 => RE.eval k1 c[t] v)
+    (P0 := fun k2 (v0 : value k2) k1 c v1 _ => RE.eval k1 c[v0] v1);
+        try match goal with 
+        | H : dec_term ?t ?k = _ |- _ =>
+              assert (G := dec_term_correct t k); rewrite H in G 
+        | H : dec_context ?ec ?k ?v = _ |- _ => 
+              assert (G := dec_context_correct ec k v); rewrite H in G
+        end;
+        subst;
+    try solve [simpl in *; congruence].
+
+    - constructor 2 with k2 c r t0...
+      assert (~dead_ckind k1) by (intro; eapply proper_death_trans; eauto).
+      apply dec_proc_eqv_dec...
+      constructor...
+    - constructor 1.
+      apply dec_proc_eqv_dec...
+      constructor...
+    - constructor 2 with k2 c r t...
+      assert (~dead_ckind k1) by (intro; eapply proper_death_trans; eauto).
+      apply dec_proc_eqv_dec... simpl.
+      rewrite G.
+      constructor...
+  Qed.
+
+
+  Lemma evalRE_imp_dec_eval :                                         forall t {k1 k2} v,
+      forall c : context k1 k2, 
+          ~dead_ckind k2 -> RE.eval k1 c[t] v -> dec_eval t c v.
+
+  Proof with eauto using (proper_death2 [.]), death_propagation2, 
+                             dec_term_next_alive, dec_context_next_alive.
+    intros t k1 k2 v c G H.
+    dependent induction H.
+        apply dec_plug in H; eauto; 
+        rewrite <- compose_empty in H.
+
+    - remember (d_val v) as d eqn: H0; revert v H0; clear G.
+      induction H using dec_Ind with
+      (P  := fun t _ _ c d _  => forall v, d = d_val v -> dec_eval t c v)
+      (P0 := fun _ v0 _ c d _ => forall v, d = d_val v -> decctx_eval v0 c v);
+      solve 
+      [ intuition eautof
+      | intros v0 H; inversion H; eauto ].
+
+    - remember (d_red r c0) as d eqn: H2; 
+      revert G k' c0 r t' v H0 H1 H2 IHeval.
+      induction H using dec_Ind with
+      (P  := fun t k1 k2 c d _ =>
+                 ~ dead_ckind k2 ->
+                 forall (k' : ckind) (c0 : context k1 k') (r : redex k') 
+                             (t' : term) (v : value k1),
+                     contract r = Some t' ->
+                     RE.eval k1 (c0) [t'] v ->
+                     d = d_red r c0 ->
+                     (forall (k3 : ckind) (c1 : context k1 k3), ~ dead_ckind k3 ->
+                      forall t0 : term, (c0) [t'] = (c1) [t0] -> dec_eval t0 c1 v) ->
+                     dec_eval t c v)
+
+      (P0 := fun k2 v0 k1 c d _ =>
+                 ~ dead_ckind k2 ->
+                 forall (k' : ckind) (c0 : context k1 k') (r : redex k') (t' : term)
+                            (v : value k1),
+                     contract r = Some t' ->
+                     RE.eval k1 (c0) [t'] v ->
+                     d = d_red r c0 ->
+                     (forall (k3 : ckind) (c1 : context k1 k3), ~ dead_ckind k3 ->
+                      forall t0 : term, (c0) [t'] = (c1) [t0] -> dec_eval t0 c1 v) ->
+                     decctx_eval v0 c v);
+
+    intros G k' c0 r' t' v' H0 H1 H2 IH;
+    inversion H2; clear H2; dep_subst...
+  Qed.
+
+
+  Axiom dec_evalRS_imp_dec_eval :              forall {t k1 k2} {v : value k1},
+      forall c : context k1 k2,
+          ~dead_ckind k2  ->  (k1 |~ c[t] →* v)  ->  dec_eval t c v.
+  Axiom dec_eval_eqv_RS :                                   forall {t k1 k2 v},
+      forall c : context k1 k2, 
+          dec_eval t c v  <->  ~dead_ckind k1 /\ (k1 |~ c[t] →* v).
+
+
+  Axiom evalRS_imp_eval :                          forall  {k t} {v : value k},
+      ~dead_ckind k  ->  (k |~ t →* v)  ->  eval k t v.
+  Axiom eval_eqv_RS :                                           forall {k t v},
+      eval k t v  <->  ~dead_ckind k /\ (k |~ t →* v).
 
   Scheme dec_Ind    := Induction for dec    Sort Prop
     with decctx_Ind := Induction for decctx Sort Prop.
