Entropy.v
@@ -1,0 +1,7 @@
+Require Import Fin.
+
+Parameters 
+(entropy  : Set)
+(draw_fin : entropy -> forall n, Fin.t n).
+
+Axiom draw_fin_correct : forall n m, exists e, draw_fin e n = m.
