reduction_languages_facts.v
@@ -1,0 +1,315 @@
+Require Import Util.
+Require Import Program.
+Require Import Eqdep.
+
+
+
+
+Module Type RED_MINI_LANG.
+
+  Parameters
+    (term         : Set)
+    (elem_context : Set)
+    (ckind        : Set)
+    (dead_ckind   : ckind -> Prop)
+    (ckind_trans  : ckind -> elem_context -> ckind)
+    (elem_plug    : term -> elem_context -> term)
+
+    (value : ckind -> Set)
+    (redex : ckind -> Set)
+    (value_to_term : forall {k}, value k -> term)
+    (redex_to_term : forall {k}, redex k -> term).
+
+  Infix "+>"           := ckind_trans (at level 50, left associativity).
+  Notation "ec :[ t ]" := (elem_plug t ec) (at level 0).
+  Coercion  value_to_term : value >-> term.
+  Coercion  redex_to_term : redex >-> term.
+
+
+
+  Inductive context (k1 : ckind) : ckind -> Set :=
+  | empty : context k1 k1
+  | ccons : forall (ec : elem_context) {k2}, context k1 k2 -> context k1 (k2+>ec).
+  Arguments empty {k1}. Arguments ccons {k1} _ {k2} _.
+
+  Notation "[.]"      := empty.
+  Notation "[.]( k )" := (@empty k).
+  Infix    "=:"       := ccons (at level 60, right associativity).
+
+  Fixpoint compose {k1 k2} (c0 : context k1 k2) 
+                      {k3} (c1 : context k3 k1) : context k3 k2 := 
+      match c0 in context _ k2' return context k3 k2' with
+      | [.]     => c1
+      | ec=:c0' => ec =: compose c0' c1
+      end.
+  Infix "~+" := compose (at level 60, right associativity).
+
+  Fixpoint plug (t : term) {k1 k2} (c : context k1 k2) : term :=
+      match c with
+      | [.]    => t 
+      | ec=:c' => plug ec:[t] c'
+      end.
+  Notation "c [ t ]" := (plug t c) (at level 0).
+
+
+
+  Axioms
+    (death_propagation : 
+         forall k, dead_ckind k -> forall ec, dead_ckind (k+>ec))
+
+    (proper_death : 
+         forall k, dead_ckind k -> ~ exists (r : redex k), True)
+
+    (value_trivial1 : 
+         forall {k} (v : value k) ec {t}, 
+             ~dead_ckind (k+>ec) -> ec:[t] = v -> 
+                 exists (v' : value (k+>ec)), t = v').
+
+End RED_MINI_LANG.
+
+
+
+
+
+Module RED_LANG_Facts (R : RED_MINI_LANG).
+
+  Import R.
+
+
+  (* Contexts *)
+
+  Lemma ccons_inj : 
+      forall ec {k1 k2} (c : context k1 k2) ec' {k2'} (c' : context k1 k2'), 
+          k2 +> ec = k2' +> ec' -> ec=:c ~= ec'=:c' ->
+          ec = ec' /\ k2 = k2' /\ c ~= c'.
+  Proof.
+    intros.
+    assert (H1 := JMeq_eq_depT _ _ _ _ _ _ H H0).
+    assert (H2 := eq_dep_eq_sigT _ _ _ _ _ _ H1). 
+    inversion H2; subst.
+    dep_subst.
+    auto.
+  Qed.
+
+
+  Ltac inversion_ccons H :=
+
+      match type of H with ?ec1 =: ?c1  ~=  ?ec2 =: ?c2 => 
+
+      let H0 := fresh in 
+      assert (H0 : eq_dep _ _ _ (ec1=:c1) _ (ec2=:c2));
+
+      [ apply JMeq_eq_depT; eauto
+
+      | inversion H0; dep_subst; clear H0 ]
+
+      end.
+
+
+  Lemma plug_empty : forall t k, [.](k)[t] = t.
+  Proof. intuition. Qed.
+
+
+  Lemma compose_empty : forall {k1 k2} (c : context k1 k2), c = c ~+ [.].
+  Proof.
+    induction c.
+    - trivial.
+    - simpl; rewrite <- IHc; trivial.
+  Qed.
+
+
+  Lemma plug_compose  : 
+      forall {k1 k2 k3} (c0 : context k1 k2) (c1 : context k3 k1) t, 
+          (c0 ~+ c1)[t] = c1[c0[t]].
+  Proof.
+    induction c0; intros.
+    - auto.
+    - apply IHc0.
+  Qed.
+
+
+  Lemma context_cons_snoc : forall ec0 {k1 k2} (c0 : context k1 k2),
+                                exists ec1 c1, (ec0=:c0) = (c1~+ec1=:[.]).
+  Proof.
+    intros; revert ec0.
+    induction c0; intros.
+    - exists ec0; eexists [.]; trivial.
+    - destruct IHc0 with ec as (ec1, (c1, IH)).
+      exists ec1; eexists (ec0=:c1); rewrite IH; trivial.
+  Qed.
+
+
+  (* Death *)
+
+  Lemma death_propagation2 : 
+      forall k ec, ~dead_ckind (k+>ec) -> ~dead_ckind k.
+
+  Proof. eauto using death_propagation. Qed.
+
+
+  Lemma dead_context_dead : 
+      forall {k1 k2}, context k1 k2 -> dead_ckind k1 -> dead_ckind k2.
+
+  Proof with auto.
+    intros ? ? c H; revert c.
+    induction 1.
+    - trivial.
+    - apply death_propagation...
+  Qed.
+
+
+  Lemma proper_death_trans :
+      forall k1, dead_ckind k1 ->
+          ~ exists {k2} (c : context k1 k2) (r : redex k2), True.
+
+  Proof with auto.
+    intros k1 H [k2 [c [ r _]]].
+    eapply proper_death.
+    - apply (dead_context_dead c)...
+    - eauto.
+  Qed.
+
+
+  Lemma proper_death2 : 
+      forall {k1 k2}, context k1 k2 -> redex k2 -> ~ dead_ckind k1.
+
+  Proof with eauto.
+    intros k1 k2 c r H.
+    apply (proper_death_trans k1)...
+  Qed.
+
+
+
+
+  (* Values *)
+
+  Lemma value_trivial : forall {k} (v : value k) {k'} (c : context k k') t, 
+                            ~dead_ckind k' -> c[t] = v -> exists (v' : value k'), t = v'.
+
+  Proof.
+    intros k v k' c t; revert t.
+    induction c;
+        intros t H H0.
+    - eauto.
+    - destruct (IHc ec:[t]) as [v' H1];
+      try solve 
+      [ eauto using death_propagation2 
+      | try rec_subst H1; eauto using value_trivial1, death_propagation2 ].
+  Qed.
+
+End RED_LANG_Facts.
+
+
+
+
+Module Type RED_MINI_LANG_WD <: RED_MINI_LANG.
+
+  Include RED_MINI_LANG.
+
+  Inductive decomp k : Set :=
+  | d_red : forall {k'}, redex k' -> context k k' -> decomp k
+  | d_val : value k -> decomp k.
+  Arguments d_val {k} _. Arguments d_red {k} {k'} _ _.
+
+  Definition decomp_to_term {k} (d : decomp k) :=
+      match d with
+      | d_val v   => value_to_term v
+      | d_red _ r c => c[r]
+      end.
+  Coercion decomp_to_term : decomp >-> term.
+
+  Definition dec (t : term) k (d : decomp k) : Prop := 
+      ~dead_ckind k /\ t = d.
+
+End RED_MINI_LANG_WD.
+
+
+
+Module RedDecProcEqvDec (R : RED_MINI_LANG_WD).
+
+  Module RF := RED_LANG_Facts R.
+  Import R RF.
+
+
+  Section S.
+
+  Variable dec_proc : forall {k1 k2}, term -> context k1 k2 -> decomp k1 -> Prop.
+  Arguments dec_proc {k1 k2} _ _ _.
+
+
+  Hypotheses
+  (dec_proc_correct :                             forall t {k1 k2} (c : context k1 k2) d,
+       dec_proc t c d -> c[t] = d)
+
+  (dec_proc_plug :      forall {k1 k2} (c : context k1 k2) {k3} (c0 : context k3 k1) t d, 
+       ~dead_ckind k2 -> dec_proc c[t] c0 d -> dec_proc t (c ~+ c0) d)
+
+  (dec_proc_plug_rev :  forall {k1 k2} (c : context k1 k2) {k3} (c0 : context k3 k1) t d, 
+       dec_proc t (c ~+ c0) d -> dec_proc c[t] c0 d)
+
+  (dec_proc_redex_self :             forall {k2} (r : redex k2) {k1} (c : context k1 k2),
+       dec_proc r c (d_red r c))
+
+  (dec_proc_value_self :                                        forall {k} (v : value k), 
+       ~dead_ckind k -> dec_proc v [.] (d_val v)).
+
+  (*dec_proc_alive :                 forall t {k1 k2} (c : context k1 k2) (d : decomp k1),
+       dec_proc t c d -> ~dead_ckind k1*)
+
+
+
+  Theorem dec_proc_eqv_dec :                      forall t {k1 k2} (c : context k1 k2) d, 
+      ~dead_ckind k2 -> (dec_proc t c d <-> dec c[t] k1 d).
+
+  Proof with eauto using (proper_death2 [.]), dead_context_dead.
+    intros; split; intro.
+    - split; [|apply dec_proc_correct]...
+    - destruct H0 as [H1 H0].
+      rewrite (compose_empty c).
+      apply dec_proc_plug...
+      rewrite H0.
+      destruct d.
+      + apply dec_proc_plug_rev...
+        rewrite <- compose_empty.
+        apply dec_proc_redex_self.
+      + apply dec_proc_value_self...
+  Qed.
+
+  End S.
+
+End RedDecProcEqvDec.
+
+
+
+(* Facts about a deterministic red. semantics.
+
+  Lemma unique_decomposition :
+
+      forall (t : term) k1, ~ dead_ckind k1 ->  
+
+         (exists v : value k1, t = v) \/
+
+         (exists k2 (r : redex k2) (c : context k1 k2), t = c[r] /\ 
+	      forall k2' (r' : redex k2') (c' : context k1 k2'), ~ dead_ckind k2' -> 
+                  t = c'[r'] -> k2' = k2 /\ r ~= r' /\ c ~= c').
+
+  Proof.
+    intros t k1 H.
+    destruct (dec_total t k1 H) as (d, H0); destruct H0.
+    destruct d.
+    - right.
+      exists k' r c.
+      split. apply (dec_correct H0).
+      intros k2' r' c' H1 H2.
+      assert (d_red r c = d_red r' c').
+      eapply dec_is_function. constructor.
+    apply H0.
+    subst.
+    apply dec_plug_rev. auto.
+    rewrite <- compose_empty.
+    apply dec_redex_self.
+    inversion H3; dep_subst.
+    auto.
+    - left. exists v. apply (dec_correct H0).
+  Qed. *)
+
