refocusing_machine_facts.v
@@ -1,177 +1,535 @@
 Require Import Util.
 Require Import Program.
 Require Import refocusing_semantics.
-Require Import refocusing_natural_semantics.
 Require Import refocusing_machine.
-Require Import reduction_semantics_facts.
-Require Import refocusing_semantics_facts.
-Require Import refocusing_natural_semantics_facts.
+Require Import reduction_languages_facts reduction_semantics_facts 
+                   refocusing_semantics_facts.
 
 
 
 
-Module RefEvalApplyMachine_Facts (R : RED_LANG) (RS : RED_REF_SEM R) 
-                                        (EAM : REF_EVAL_APPLY_MACHINE R RS).
+Module RefEvalApplyMachine_Facts (R : RED_REF_SEM) (EAM : REF_EVAL_APPLY_MACHINE R).
 
-  Module RNS  := RefNaturalSem R RS.
-  Module RNSF := RefNaturalSem_Facts R RS RNS.
-  Import R.
-  Import RS.ST.
+  Module RF := RED_LANG_Facts R.
+  Import R.R R RF.
+
+  Notation "c1 >> c2" := (init_ckind |~ c1 → c2) (no associativity, at level 70).
+  Notation "k |~ c1 >> c2" := (k |~ c1 → c2)     
+                                         (no associativity, at level 70, c1 at level 69).
+
+
+  Import ST.
   Import EAM.
 
 
+  Local Hint Constructors EAM.trans clos_trans_1n.
 
-  Local Hint Constructors EAM.trans EAM.trans_close.
-  Local Hint Constructors RNS.dec RNS.decctx.
+  Theorem am_correct :                                                      forall c1 c2,
+      c1 → c2 -> decompile c1 = decompile c2 \/ decompile c1 >> decompile c2.
 
-
-  Lemma dec_RNS_eqv_EAM : forall {t k1 k2} (c : context k1 k2) {v}, 
-                              RNS.dec t c v <-> c_eval t c →+ c_apply [.] v.
   Proof with eauto.
-    intros t k1 k2 c v; split; intro H.
-
-  (* -> *) {
-    induction H using RNS.dec_Ind with
-    (P := fun t _ _ c v  (_ : RNS.dec t c v) => 
-              c_eval t c  →+ c_apply [.] v)
-    (P0:= fun k2 v k1 c v' (_ : RNS.decctx v c v') => 
-              c_apply c v →+ c_apply [.] v' \/ k1 = k2 /\ [.](k1) ~= c /\ v ~=v');
-
-    intuition; dep_subst...
-  }
-
-  (* <- *) {
-    revert t k2 c H.
-
-    cut (forall st, st →+ c_apply [.] v -> 
-         match st with 
-         | c_eval t k1' _ c   => k1 = k1' -> forall v', v ~= v' -> RNS.dec t c v'
-         | c_apply k1' _ c v0 => k1 = k1' -> forall v', v ~= v' -> RNS.decctx v0 c v'
-         end).
-    { intros H t k2 c H0; apply (H _ H0)... }
-
-    intros st H.
-
-    dependent induction H;
-        match goal with H : _ → _ |- _ => 
-              dependent_destruction2 H end;
-        match goal with 
-        | H : dec_term _ ?k = _ |- _=> 
-              assert (~ dead_ckind k);
-              [ intro; rewrite dec_term_from_dead in H; solve[eauto] 
-              | ]
-        | H : dec_context _ ?k _ = _ |- _=> 
-              assert (~ dead_ckind k);
-              [ intro; rewrite dec_context_from_dead in H; 
-                solve [eauto using death_propagation] 
-              | ]
+    intros c1 c2 H.
+    inversion H; subst;
+        try match goal with 
+        | H : dec_term ?t ?k = _ |- _ =>
+              assert (G := dec_term_correct t k);
+              rewrite H in G
+        | H : dec_context ?ec ?k ?v = _ |- _ =>
+              assert (G := dec_context_correct ec k v);
+              rewrite H in G
         end;
-
-    intros; dep_subst...
-  }
+    try solve [left; simpl; congruence].
+    - right. 
+      unfold reduce, dec. 
+      exists k c r t0.
+      intuition.
+      + eapply proper_death_trans...
+      + simpl.
+        congruence.
+    - right.
+      unfold reduce, dec.
+      exists k c r t.
+      intuition.
+      + eapply proper_death_trans...
+      + simpl.
+        congruence.
   Qed.
 
+Require Import Vector.
 
 
-  Lemma decctx_RNS_eqv_EAM : 
-      forall {k1 k2} (c : context k1 k2) {v0 v1}, 
-          RNS.decctx v0 c v1 <-> c_apply c v0 →+ c_apply [.] v1 \/
-                                 c_apply c v0 = c_apply [.] v1 /\ ~dead_ckind k1.
+Fixpoint fin_lift {n} (m : Fin.t n) := match m with
+| Fin.F1 n => @Fin.F1 (S n)
+| Fin.FS _ m => Fin.FS (fin_lift m)
+end.
+Fixpoint fin_to_nat {n} (m : Fin.t n) := match m with
+| Fin.F1 _   => 0
+| Fin.FS _ m => S (fin_to_nat m)
+end.
 
+Coercion fin_lift : Fin.t >-> Fin.t.
+Coercion fin_to_nat : Fin.t >-> nat.
+
+Arguments cons {A} _ {n} _.
+
+Import VectorNotations.
+Infix "++" := append.
+
+
+  Lemma dec_proc_sim :               forall t {k1 k2} (d : decomp k1) (c : context k1 k2) 
+                                                                   (c0 : context ick k1),
+      dec_proc t c d ->
+          exists n (sts : Vector.t conf n),
+          (**)Forall (fun st => decompile st = (c~+c0)[t]) sts /\
+          (**)match d with 
+              | d_val v      => last (c_eval t (c ~+ c0) :: sts) = c_apply c0 v 
+              | d_red k r c' => last (c_eval t (c ~+ c0) :: sts) = c_eval r (c'~+c0) /\
+                                dec_term r k = in_red r                              \/
+                                exists ec v, dec_context ec k v = in_red r           /\
+                                last (c_eval t (c ~+ c0) :: sts) = c_apply (ec=:c'~+c0) v
+              end /\
+          (**)forall m : Fin.t n, (c_eval t (c~+c0) :: sts)[@m] → sts[@m].
   Proof with eauto.
-    intros k1 k2 c v0 v1; split; intro H.
+    intros t k1 k2 d c c0 H.
+    induction H using dec_proc_Ind with
+    (P := fun k2 t (c : context k1 k2) d (_ : dec_proc t c d) =>
+exists (n : nat) (sts : Vector.t configuration n),
+  Forall (fun st : configuration => decompile st = (c ~+ c0) [t]) sts /\
+match d with 
+              | d_val v      => last (c_eval t (c ~+ c0) :: sts) = c_apply c0 v 
+              | d_red k r c' => last (c_eval t (c ~+ c0) :: sts) = c_eval r (c'~+c0) /\
+                                dec_term r k = in_red r                              \/
+                                exists ec v, dec_context ec k v = in_red r           /\
+                                last (c_eval t (c ~+ c0) :: sts) = c_apply (ec=:c'~+c0) v
+              end /\
+  (forall m : Fin.t n, (c_eval t (c ~+ c0) :: sts)[@m] → sts[@m]))
 
-  (* -> *) {
-    induction H using RNS.decctx_Ind with
-    (P := fun t _ _ c v  (_ : RNS.dec t c v)     => 
-              c_eval t c  →+ c_apply [.] v)
-    (P0:= fun k2 v k1 c v' (_ : RNS.decctx v c v') => 
-              c_apply c v →+ c_apply [.] v' \/ 
-              c_apply c v = c_apply [.] v' /\ ~dead_ckind k1);
+    (P0 := fun k2 (v' : R.value k2) (c : context k1 k2) d _ =>
+exists (n : nat) (sts : Vector.t configuration n),
+  Forall (fun st : configuration => decompile st = (c ~+ c0) [v']) sts /\
+match d with 
+              | d_val v      => last (c_apply (c ~+ c0) v' :: sts) = c_apply c0 v 
+              | d_red k r c' => last (c_apply (c ~+ c0) v' :: sts) = c_eval r (c'~+c0) /\
+                                dec_term r k = in_red r                              \/
+                                exists ec v, dec_context ec k v = in_red r           /\
+                                last (c_apply (c ~+ c0) v' :: sts) = c_apply (ec=:c'~+c0) v
+              end /\
+  (forall m : Fin.t n, (c_apply (c ~+ c0) v' :: sts)[@m] → sts[@m]));
 
+         subst;
+
+      try destruct IHdec_proc as [n [sts [H0 [H1 H2]]]]; auto;
+      repeat match goal with
+      | H : dec_term ?t ?k = _ |- _ => 
+            assert (G := dec_term_correct t k);
+            rewrite H in G
+      | H : dec_context ?ec ?k ?v = _ |- _ => 
+            assert (G := dec_context_correct ec k v);
+            rewrite H in G
+      end;
+      subst;
+
+  [ exists 0 (nil configuration)
+  | exists (S n) (c_apply (c~+c0) v :: sts)
+  | exists (S n) (c_eval t0 (ec =: c~+c0) :: sts) 
+  | exists 0 (nil configuration)
+  | exists 0 (nil configuration)
+  | exists (S n) (c_apply (c ~+ c0) v0 :: sts)
+  | exists (S n) (c_eval t (ec0 =: c ~+ c0) :: sts) ];
+
+  solve [ split;
+  [ constructor; simpl; try rewrite G; auto
+  | split;
+  [ eauto
+  | intro m;
+    dependent_destruction2 m; 
     solve
-    [ intuition; dep_subst; eauto
-    | destruct IHdecctx as [H0 | [H0 H1]]; inversion H0; dep_subst; eauto ].
-
-  }
-
-  (* <- *) {
-    revert k2 v0 c H.
-
-    cut (forall st, st →+ c_apply [.] v1 -> 
-         match st with 
-         | c_eval t k1' _ c   => k1 = k1' -> forall v', v1 ~= v' -> RNS.dec t c v'
-         | c_apply k1' _ c v0 => k1 = k1' -> forall v', v1 ~= v' -> RNS.decctx v0 c v'
-         end).
-    { intros H t k2 c H0.
-      destruct H0 as [H0 | [H0 H1]]. 
-      - apply (H _ H0)...
-      - inversion H0; dep_subst... }
-
-    intros st H.
-    dependent induction H;
-        match goal with H : _ → _ |- _ => 
-              dependent_destruction2 H end;
-        match goal with 
-        | H : dec_term _ ?k = _ |- _=> 
-              assert (~ dead_ckind k);
-              [ intro; rewrite dec_term_from_dead in H; solve[eauto] 
-              | ]
-        | H : dec_context _ ?k _ = _ |- _=> 
-              assert (~ dead_ckind k);
-              [ intro; rewrite dec_context_from_dead in H; 
-                solve [eauto using death_propagation] 
-              | ]
-        end;
-
-    intros; dep_subst...
-  }
+    [ simpl; eauto 
+    | apply H2 ]
+  ] ] ].
   Qed.
 
 
+  Lemma decctx_proc_sim :                         forall {k1 k2} v' d (c : context k1 k2) 
+                                                                   (c0 : context ick k1),
+      decctx_proc v' c d ->
+          exists (n : nat) (sts : Vector.t configuration n),
+              Forall (fun st => decompile st = (c ~+ c0) [v']) sts /\
+              match d with 
+              | d_val v      => last (c_apply (c ~+ c0) v' :: sts) = c_apply c0 v 
+              | d_red k r c' => last (c_apply (c ~+ c0) v' :: sts) = c_eval r (c'~+c0) /\
+                                dec_term r k = in_red r                              \/
+                                exists ec v, dec_context ec k v = in_red r           /\
+                                last (c_apply (c ~+ c0) v' :: sts) = c_apply (ec=:c'~+c0) v
+              end /\
+  (forall m : Fin.t n, (c_apply (c ~+ c0) v' :: sts)[@m] → sts[@m]).
+  Proof with eauto.
+    intros k1 k2 v' d c c0 H.
+    induction H using decctx_proc_Ind with
+    (P := fun k2 t (c : context k1 k2) d (_ : dec_proc t c d) =>
+exists (n : nat) (sts : Vector.t configuration n),
+  Forall (fun st : configuration => decompile st = (c ~+ c0) [t]) sts /\
+match d with 
+              | d_val v      => last (c_eval t (c ~+ c0) :: sts) = c_apply c0 v 
+              | d_red k r c' => last (c_eval t (c ~+ c0) :: sts) = c_eval r (c'~+c0) /\
+                                dec_term r k = in_red r                              \/
+                                exists ec v, dec_context ec k v = in_red r           /\
+                                last (c_eval t (c ~+ c0) :: sts) = c_apply (ec=:c'~+c0) v
+              end /\
+  (forall m : Fin.t n, (c_eval t (c ~+ c0) :: sts)[@m] → sts[@m]))
 
-  Lemma eval_RNS_eqv_EAM : forall {t v}, RNS.eval t v <-> EAM.eval t v.
+    (P0 := fun k2 (v' : R.value k2) (c : context k1 k2) d _ =>
+exists (n : nat) (sts : Vector.t configuration n),
+  Forall (fun st : configuration => decompile st = (c ~+ c0) [v']) sts /\
+match d with 
+              | d_val v      => last (c_apply (c ~+ c0) v' :: sts) = c_apply c0 v 
+              | d_red k r c' => last (c_apply (c ~+ c0) v' :: sts) = c_eval r (c'~+c0) /\
+                                dec_term r k = in_red r                              \/
+                                exists ec v, dec_context ec k v = in_red r           /\
+                                last (c_apply (c ~+ c0) v' :: sts) = c_apply (ec=:c'~+c0) v
+              end /\
+  (forall m : Fin.t n, (c_apply (c ~+ c0) v' :: sts)[@m] → sts[@m]));
+
+         subst;
+
+      try destruct IHdecctx_proc as [n [sts [H0 [H1 H2]]]]; auto;
+      repeat match goal with
+      | H : dec_term ?t ?k = _ |- _ => 
+            assert (G := dec_term_correct t k);
+            rewrite H in G
+      | H : dec_context ?ec ?k ?v = _ |- _ => 
+            assert (G := dec_context_correct ec k v);
+            rewrite H in G
+      end;
+      subst;
+
+  [ exists 0 (nil configuration)
+  | exists (S n) (c_apply (c~+c0) v :: sts)
+  | exists (S n) (c_eval t0 (ec =: c~+c0) :: sts) 
+  | exists 0 (nil configuration)
+  | exists 0 (nil configuration)
+  | exists (S n) (c_apply (c ~+ c0) v0 :: sts)
+  | exists (S n) (c_eval t (ec0 =: c ~+ c0) :: sts) ];
+
+  solve [ split;
+  [ constructor; simpl; try rewrite G; auto
+  | split;
+  [ eauto
+  | intro m;
+    dependent_destruction2 m; 
+    solve
+    [ simpl; eauto 
+    | apply H2 ]
+  ] ] ].
+  Qed.
+
+
+  Lemma mid_ccons_as_append :                      forall {k1 k2} (c1 : context k1 k2) ec
+                                                         {k3} (c2 : context (k2+>ec) k3),
+      c2 ~+ ec =: c1 = c2 ~+ (ec =: [.]) ~+ c1.
+
   Proof.
-    intros t v; split; intro H;
-    solve 
-    [ dependent destruction H; constructor; apply dec_RNS_eqv_EAM; eauto ].
+    intros k1 k2 c1 ec k3 c2.
+    induction c2;
+    solve [ auto ].
   Qed.
 
 
+  Lemma append_assoc : forall {k4 k3} (c1 : context k3 k4) {k2} (c2 : context k2 k3)
+                         {k1} (c3 : context k1 k2),
+      c1 ~+ c2 ~+ c3 = (c1 ~+ c2) ~+ c3.
+  Proof.
+    induction c1; intros; 
+    solve [simpl; f_equal; eauto].
+  Qed.
 
-  Theorem dec_iter_composition :
-      forall {t k1 k2} {c : context k1 k2} {v},
-          (exists d, RS.dec t c d /\ RS.iter d v) <-> c_eval t c →+ c_apply [.] v.
+
+  Lemma ccons_append_empty_self_JM : forall {k1 k2} (c1 : context k1 k2) {k3} (c2 : context k2 k3),
+      k2 = k3 -> c1 ~= c2 ~+ c1 -> c2 ~= [.](k2).
+
+  Proof with eauto.
+    intros k1 k2 c1.
+    induction c1; intros k3 c2 H H0;
+      destruct c2...
+    - discriminateJM H0.
+    - exfalso.
+      simpl in H0.
+      inversion_ccons H0; clear H5 x.
+      assert (H1 : c2 ~+ ec0 =: [.](k0) ~= [.](k0)). 
+      {
+          eapply IHc1...
+          rewrite <- append_assoc. 
+          rewrite <- (mid_ccons_as_append c1 ec0 c2).
+          rewrite <- x0.
+          reflexivity.
+      }
+      revert H1. clear. revert c2.
+      cut (forall k (c : context (k0 +> ec0) k), k = k0 -> ~ (c ~+ ec0 =: [.](k0) ~= [.](k0))).
+      intro. intros. eapply H. reflexivity. exact H1.
+      intros k c G H.
+      destruct c;
+      discriminateJM H.
+  Qed.
+
+
+  Lemma ccons_append_empty_self : forall {k1 k2} (c1 : context k1 k2) (c2 : context k2 k2),
+      c1 = c2 ~+ c1 -> c2 = [.](k2).
+
+  Proof with eauto. 
+    intros.
+    cut (c2 ~= [.](k2)).
+    { intro H0; rewrite H0... }
+    eapply ccons_append_empty_self_JM with c1...
+    rewrite <- H.
+    solve [trivial].
+  Qed.
+
+
+  Lemma local1 : forall {n} (sts : Vector.t configuration n) st1 st2,
+  (*1*)(forall m : Fin.t n, (st1 :: sts)[@m] → sts[@m]) ->
+  (*2*)last (st1 :: sts) → st2 ->
+
+      forall m : Fin.t (n + 1), (st1 :: sts ++ [st2])[@m] → (sts ++ [st2])[@m].
 
   Proof.
-    etransitivity; eauto using dec_RNS_eqv_EAM, RNSF.dec_iter_composition.
+    intros n sts st1 st2 H H0. revert st1 H H0.
+    induction sts; intros.
+    - dependent destruction m.
+      + auto.
+      + inversion m.
+    - dependent destruction m.
+      + apply (H Fin.F1).
+      + apply IHsts.
+        * intro m0. apply (H (Fin.FS m0)).
+        * auto.
   Qed.
 
 
 
-  Theorem decctx_iter_composition : forall {k1 k2} {c : context k1 k2} {v0 v1},
+  Theorem am_context_complete :                  forall t1 t2 {k} (c : context ick k) st,
+      k |~ t1 >> t2 -> decompile st = c[t1] -> 
+          exists n (sts : Vector.t configuration n) st,
+          (**)Forall (fun st => decompile st = c[t1]) sts /\
+          (**)decompile st = c[t2]                        /\
+          (**)forall m : Fin.t (n+1), 
+                  (c_eval t1 c :: sts ++ [st])[@m] → (sts ++ [st])[@m].
 
-      (exists d, RS.decctx v0 c d /\ RS.iter d v1) <-> 
+  Proof with eauto.
+    intros t1 t2 k c st H H0.
+    destruct H as [k2 [c2 [r [t [[H H1] [H2 H3]]]]]].
+    assert (H4 : dec c[t1] ick (d_red r (c2~+c))).
+    {
+        constructor;
+        solve [subst; simpl; eauto using dead_context_dead, plug_compose].
+    }
+    assert (~dead_ckind k2) by eauto using (proper_death2 [.]).
+    apply dec_proc_eqv_dec in H4...
+    destruct (dec_proc_sim _ _ _ [.] H4) as [n [sts [G [ [[G0 G1] | [ec [v [G1 G0]]]] G2] ]]];
+        rewrite <- (compose_empty c) in *;
+        rewrite <- (compose_empty (c2~+c)) in *;
+        exists n sts (c_eval t (c2 ~+ c));
+    (
+        split;
+        [ auto
+        | split;
+        [ simpl; rewrite plug_compose; congruence
+        | apply local1; eauto;
+          unfold configuration; (*sic*)
+          rewrite G0
+        ] ]
+    );
+    [ econstructor 1 | econstructor 4 ]...
+  Qed.
 
-      c_apply c v0 →+ c_apply [.] v1 \/
-      c_apply c v0 = c_apply [.] v1 /\ ~dead_ckind k1.
+
+
+  Corollary am_complete :                                                forall t1 t2 st,
+      t1 >> t2 -> decompile st = t1 -> 
+          exists n (sts : Vector.t configuration n) st,
+          (**)Forall (fun st => decompile st = t1) sts /\
+          (**)decompile st = t2                        /\
+          (**)forall m : Fin.t (n+1), 
+                  (c_eval t1 [.] :: sts ++ [st])[@m] → (sts ++ [st])[@m].
+  Proof with eauto.
+    intros.
+    apply (am_context_complete t1 t2 [.] st)...
+  Qed.
+
+
+
+  Axiom init_ckind_alive : ~dead_ckind ick.
+
+
+  Lemma vec_last_by_index : forall {T n} (v : Vector.t T (S n)) (H : n < S n), 
+      last v = v[@ Fin.of_nat_lt H].
 
   Proof.
-    etransitivity; eauto using decctx_RNS_eqv_EAM, RNSF.decctx_iter_composition.
+    intros.
+    dependent induction v.
+    destruct v.
+    - auto.
+    - apply (IHv n (h0 :: v)); auto.
   Qed.
 
 
 
-  Theorem eval_preservation : forall {t v}, RS.eval t v <-> EAM.eval t v.
+  Lemma no_silent_loops_eval : forall t {k} (c : context ick k),
+      ~ exists sts : nat -> configuration, 
+          sts 0 = c_eval t c /\
+          forall n, sts n → sts (S n) /\ ~ decompile (sts n) >> decompile (sts (S n)).
 
-  Proof. etransitivity; eauto using RNSF.eval_preserved, eval_RNS_eqv_EAM. Qed.
+  Proof with eauto using init_ckind_alive.
+    intros t k c [sts [H H0]].
+    destruct (decompose c[t] ick) as [d H1]...
+    assert (H2 : ~dead_ckind k).
+    { intro H2; apply dec_term_from_dead with t k in H2. 
+      destruct (H0 0) as [H3 _].
+      rewrite H in H3.
+      inversion H3; congruence. }
+    apply dec_proc_eqv_dec in H1...
+    destruct (dec_proc_sim _ _ _ [.] H1) as [n [sts' [H3 [H4 H5]]]].
+    rewrite <- (compose_empty c) in *.
+    cut (forall m, (sts 0 :: sts')[@m] = sts m).
+    {
+        intro H6.
+        destruct d.
+        - rewrite <- (compose_empty c0) in *.
+          destruct H4 as [[G G0] | [ec [v [G0 G]]]];
+              assert (H7 : n < S n) by eauto with arith;
+              rewrite vec_last_by_index with _ H7 in G;
+              rewrite <- H in G;
+              rewrite H6 in G;
+              destruct (H0 (Fin.of_nat_lt H7)) as [H8 H9];
+              rewrite G in H8;
+              dependent destruction H8; dep_subst; try congruence;
+              replace r0 with r in * by congruence;
+              apply H9.
+          + rewrite G; rewrite <- x.
+            simpl.
+            exists k' c0 r t1.
+            intuition unfold dec... 
+          + rewrite G; rewrite <- x.
+            simpl.
+            assert (H10 := dec_context_correct ec k' v); rewrite H4 in H10.
+            rewrite H10.
+            exists k' c0 r t0.
+            intuition unfold dec...
+        - assert (H7 : n < S n) by eauto with arith;
+          rewrite vec_last_by_index with _ H7 in H4.
+          rewrite <- H in H4.
+          rewrite H6 in H4.
+          destruct (H0 (Fin.of_nat_lt H7)) as [H8 _].
+          rewrite H4 in H8.
+          inversion H8.
+    }
+    rewrite <- H in H5.
+    clear t k c H d H1 H2 H3 H4. 
+    remember (sts 0) as st. revert sts H0 st Heqst H5.
+    induction sts'; intros.
+    - dependent destruction m.
+      + auto. 
+      + inversion m.
+    - dependent destruction m. 
+      + auto.
+      + eapply (IHsts' (fun n => sts (S n)))...
+        * destruct (H0 0) as [H1 _].
+          assert (H2 := H5 Fin.F1); simpl in H2.
+          rewrite <- Heqst in H1.
+          rewrite trans_computable in H1, H2.
+          destruct H1, H2.
+          unfold next_conf in H, H1; congruence.
+        * intro m0. apply (H5 (Fin.FS m0)).
+  Qed.
+
+
+  Lemma no_silent_loops_apply : forall {k} v (c : context ick k),
+      ~ exists sts : nat -> configuration, 
+          sts 0 = c_apply c v /\
+          forall n, sts n → sts (S n) /\ ~ decompile (sts n) >> decompile (sts (S n)).
+
+  Proof with eauto using init_ckind_alive.
+    intros k v c [sts [H H0]].
+    destruct (decompose c[v] ick) as [d H1]...
+    assert (H2 : ~dead_ckind k).
+    { destruct (H0 0) as [H3 _].
+      rewrite H in H3.
+      inversion H3; dep_subst;
+          intro H2; apply dec_context_from_dead with ec k0 v in H2; congruence. }
+    apply dec_proc_eqv_dec in H1...
+    apply dec_proc_val_eqv_decctx in H1.
+    destruct (decctx_proc_sim _ _ _ [.] H1) as [n [sts' [H3 [H4 H5]]]].
+    rewrite <- (compose_empty c) in *.
+    cut (forall m, (sts 0 :: sts')[@m] = sts m).
+    {
+        intro H6.
+        destruct d.
+        - rewrite <- (compose_empty c0) in *.
+          destruct H4 as [[G G0] | [ec [v0 [G0 G]]]];
+              assert (H7 : n < S n) by eauto with arith;
+              rewrite vec_last_by_index with _ H7 in G;
+              rewrite <- H in G;
+              rewrite H6 in G;
+              destruct (H0 (Fin.of_nat_lt H7)) as [H8 H9];
+              rewrite G in H8;
+              dependent destruction H8; dep_subst; try congruence;
+              replace r0 with r in * by congruence;
+              apply H9.
+          + rewrite G; rewrite <- x.
+            simpl.
+            exists k' c0 r t0.
+            intuition unfold dec... 
+          + rewrite G; rewrite <- x.
+            simpl.
+            assert (H10 := dec_context_correct ec k' v0); rewrite H4 in H10.
+            rewrite H10.
+            exists k' c0 r t.
+            intuition unfold dec...
+        - assert (H7 : n < S n) by eauto with arith;
+          rewrite vec_last_by_index with _ H7 in H4.
+          rewrite <- H in H4.
+          rewrite H6 in H4.
+          destruct (H0 (Fin.of_nat_lt H7)) as [H8 _].
+          rewrite H4 in H8.
+          inversion H8.
+    }
+    rewrite <- H in H5.
+    clear v k c H d H1 H2 H3 H4. 
+    remember (sts 0) as st. revert sts H0 st Heqst H5.
+    induction sts'; intros.
+    - dependent destruction m.
+      + auto. 
+      + inversion m.
+    - dependent destruction m. 
+      + auto.
+      + eapply (IHsts' (fun n => sts (S n)))...
+        * destruct (H0 0) as [H1 _].
+          assert (H2 := H5 Fin.F1); simpl in H2.
+          rewrite <- Heqst in H1.
+          rewrite trans_computable in H1, H2.
+          destruct H1, H2.
+          unfold next_conf in H, H1; congruence.
+        * intro m0. apply (H5 (Fin.FS m0)).
+  Qed.
+  
+
+  Theorem no_silent_loops :
+      ~ exists sts : nat -> configuration,
+          forall n, sts n → sts (S n) /\ ~ decompile (sts n) >> decompile (sts (S n)).
+
+  Proof with eauto.
+    intros [sts H].
+    remember (sts 0) as st.
+    destruct st.
+    - apply (no_silent_loops_eval t c)...
+    - apply (no_silent_loops_apply v c)...
+  Qed.
 
 End RefEvalApplyMachine_Facts.
 
 
 
 
-Module PushEnterMachine_Facts (R : RED_LANG) (PERS : PE_RED_REF_SEM R) 
+(*Module PushEnterMachine_Facts (R : RED_LANG) (PERS : PE_RED_REF_SEM R) 
                                         (PEM : REF_PUSH_ENTER_MACHINE R PERS).
 
   Module PENS  := PE_RefNaturalSem R PERS.
@@ -228,4 +586,4 @@ Module PushEnterMachine_Facts (R : RED_LANG) (PERS : PE_RED_REF_SEM R)
 
   Proof. etransitivity; eauto using PENSF.eval_preserved, eval_PENS_eqv_PEM. Qed.
 
-End PushEnterMachine_Facts.
+End PushEnterMachine_Facts.*)
