refocusing_semantics_facts.v
@@ -1,48 +1,90 @@
 Require Import Util.
 Require Import Program.
 Require Import refocusing_semantics.
-Require Import reduction_semantics_facts.
+Require Import reduction_languages_facts.
+
+
+
+
+Module RED_REF_SEM_Facts (R : RED_REF_SEM).
+
+  Module RF := RED_LANG_Facts R.
+  Import R RF.
+
+
+  Lemma dec_proc_starts_alive :                   forall t {k1 k2} (c : context k1 k2) d,
+      dec_proc t c d -> ~dead_ckind k2.
+
+  Proof.
+    intros t k1 k2 c d H H0.
+    apply dec_term_from_dead with t k2 in H0.
+    assert (G := dec_term_correct t k2).
+    destruct H;
+    match goal with H : dec_term ?t ?k = _ |- _ =>
+    rewrite H in G
+    end;
+    solve [congruence].
+  Qed.
+
+
+  Lemma decctx_proc_starts_alive : forall {k2} (v : value k2) {k1} (c : context k1 k2) d,
+      decctx_proc v c d -> ~dead_ckind k2.
+
+  Proof with auto.
+    intros k2 v k1 c d H H0.
+    destruct c as [| ec k2 c].
+    - inversion H; dep_subst...
+    - apply dec_context_from_dead with ec k2 v in H0.
+      assert (G := dec_context_correct ec k2 v).
+      dependent destruction H; inversion_ccons x; dep_subst; (* WAR: unbound x *)
+      match goal with H : dec_context ?ec ?k ?v = _ |- _ =>
+      rewrite H in G
+      end;
+      solve [congruence].
+  Qed.
+
+
+
+
+End RED_REF_SEM_Facts.
 
 
 
 
 (* Refocusing semantics is deterministic. *)
 
-Module RedRefSemDet (R : RED_LANG) (RS : RED_REF_SEM R) <: DET_RED_SEM R.
+Module RedRefSemDet (R : RED_REF_SEM) <: RED_SEM_DET R.
 
-  Include RS.
-
-  Import R.
-  Module RLF := RED_LANG_Facts R.
-  Import RLF.
+  Module RF := RED_LANG_Facts R.
+  Import R RF.
 
 
-  Lemma dec_is_function : forall {t k} {d0 d1 : decomp k}, 
-                              decempty t d0 -> decempty t d1 -> d0 = d1.
+  Lemma dec_proc_is_pfunction :               forall t {k1 k2} (c : context k1 k2) d0 d1,
+      dec_proc t c d0 -> dec_proc t c d1 -> d0 = d1.
+
   Proof.
-    intros t k d0 d1 DE0 DE1.
-    dependent destruction DE0; dependent destruction DE1.
+    intros t k1 k2 c d0 d1 DE0 DE1. revert d1 DE1.
 
-    induction H using dec_Ind with 
-    (P  := fun t _ _ c d _ => forall d1, dec t c d1    -> d = d1)
-    (P0 := fun _ v _ c d _ => forall d1, decctx v c d1 -> d = d1);
+    induction DE0 using dec_proc_Ind with 
+    (P  := fun _ t c d _ => forall d1, dec_proc t c d1    -> d = d1)
+    (P0 := fun _ v c d _ => forall d1, decctx_proc v c d1 -> d = d1);
 
     intros;
 
     (* automated cases *)
     match goal with
 
-    | [ RD : (dec ?t ?c ?d), DT1 : (dec_term ?t ?k = _) |- _ ] => 
+    | [ RD : (dec_proc ?t ?c ?d), DT1 : (dec_term ?t ?k = _) |- _ ] => 
              inversion RD; dep_subst; 
              match goal with DT2 : (dec_term ?t ?k = _) |- _ => 
                  rewrite DT2 in DT1; inversion DT1 end
 
-    | [ RC : (decctx ?v (?ec=:?c) ?d), DC1 : (dec_context ?ec ?k ?v = _) |- _ ] => 
+    | [ RC : (decctx_proc ?v (?ec=:?c) ?d), DC1 : (dec_context ?ec ?k ?v = _) |- _ ] => 
              dependent_destruction2 RC; inversion_ccons x2; dep_subst;
              match goal with DC2 : (dec_context ?ec' ?k' ?v' = _) |- _ => 
                  rewrite DC2 in DC1; inversion DC1 end
 
-    | [ RC : (decctx ?v [.] ?d) |- _] => 
+    | [ RC : (decctx_proc ?v [.] ?d) |- _] => 
              dependent_destruction2 RC
 
     end;
@@ -51,7 +93,21 @@ Module RedRefSemDet (R : RED_LANG) (RS : RED_REF_SEM R) <: DET_RED_SEM R.
   Qed.
 
 
-  Lemma iter_is_function : forall {k} {d : decomp k} {v0 v1}, 
+
+  Theorem dec_is_pfunction :                             forall t {k} (d0 d1 : decomp k),
+      dec t k d0 -> dec t k d1 -> d0 = d1.
+
+  Proof with auto.
+    intros t k d0 d1 H H0.
+    assert (~dead_ckind k) by apply H.
+    rewrite <- (plug_empty t k) in H, H0.
+    apply dec_proc_eqv_dec in H...
+    apply dec_proc_eqv_dec in H0...
+    eauto 10 using dec_proc_is_pfunction.
+  Qed.
+
+
+(*  Lemma iter_is_function : forall {k} {d : decomp k} {v0 v1}, 
                                iter d v0 -> iter d v1 -> v0 = v1.
   Proof with eauto.
     intros k d v0 v1.
@@ -69,10 +125,34 @@ Module RedRefSemDet (R : RED_LANG) (RS : RED_REF_SEM R) <: DET_RED_SEM R.
   Proof with eauto.
     intros t v0 v1 H H0.
     dependent destruction H.
-    dependent destruction H1.
-    eapply iter_is_function.
-    - apply H0.
-    - erewrite dec_is_function...
-  Qed.
+    dependent destruction H0.
+    dependent induction H.
+    - dependent destruction H0.
+      + auto using value_to_term_injective.
+      + destruct H as [k [c [r [t [H _]]]]].
+        apply dec_correct in H.
+        destruct (value_trivial v c r) as [v1 H1]; 
+            eauto using (proper_death2 [.] r).
+        symmetry in H1.
+        apply value_redex in H1.
+        autof.
+    - dependent destruction H1.
+      + destruct H as [k [c [r [t [H _]]]]].
+        apply dec_correct in H.
+        destruct (value_trivial v0 c r) as [v1 H1]; 
+            eauto using (proper_death2 [.] r).
+        symmetry in H1.
+        apply value_redex in H1.
+        autof.
+      + destruct H  as [k1 [c1 [r1 [t1 [H3 [H4 H5]]]]]],
+                 H1 as [k2 [c2 [r2 [t2 [G3 [G4 G5]]]]]].
+        assert (H6 : d_red r1 c1 = d_red r2 c2).
+        { eauto using dec_is_function. }
+        inversion H6; dep_subst.
+        assert (H5 : t1 = t2).
+        { congruence. }
+        subst.
+        eauto.
+  Qed.*)
 
 End RedRefSemDet.
