rewriting_system.v
@@ -1,0 +1,17 @@
+Require Import Relations.
+
+
+
+Module Type REWRITING_SYSTEM.
+
+  Parameters
+  (configuration : Set)
+  (transition    : configuration -> configuration -> Prop).
+
+  Notation "c1 → c2"  := (transition c1 c2)              (no associativity, at level 70).
+  Notation "t1 →+ t2" := (clos_trans_1n _ transition t1 t2) 
+                                                         (no associativity, at level 70).
+  Notation "t1 →* t2" := (clos_refl_trans_1n _ transition t1 t2) 
+                                                         (no associativity, at level 70).
+
+End REWRITING_SYSTEM.
